added diagrams lemmas for closed FSIM, added the public_symbol_preserve in closed FSIM and BSIM

common/SmallstepClosed.v
@@ -98,13 +98,71 @@ Record semantics := ClosedSemantics_gen {
 
 Declare Scope closed_smallstep_scope.
 
+Section CLOSURES.
+
+Variable genv: Type.
+Variable state: Type.
+
+Variable step: genv -> state -> trace -> state -> Prop.
+
+Variable final_state: state -> int -> Prop.
+
+Inductive eventually (ge: genv): nat -> state -> (state -> Prop) -> Prop :=
+  | eventually_now: forall s (P: state -> Prop),
+      P s ->
+      eventually ge O s P
+  | eventually_later: forall n s (P: state -> Prop),
+      (forall r, ~ final_state s r) ->
+      (forall t s', step ge s t s' -> t = E0 /\ eventually ge n s' P) ->
+      eventually ge (S n) s P.
+
+Lemma eventually_one: forall ge s (P: state -> Prop),
+  (forall r, ~ final_state s r) ->
+  (forall t s', step ge s t s' -> t = E0 /\ P s') ->
+  eventually ge 1%nat s P.
+Proof.
+  intros. apply eventually_later; auto. intros.
+  apply H0 in H1.
+  intuition auto using eventually.
+Qed.
+
+Lemma eventually_trans: forall ge n1 s1 P1 n2 P2,
+  eventually ge n1 s1 P1 -> 
+  (forall s2, P1 s2 -> eventually ge n2 s2 P2) ->
+  eventually ge (n1 + n2)%nat s1 P2.
+Proof.
+  intros. revert n1 s1 H. induction n1; intros s1 EV; inv EV; simpl.
+- apply H0; assumption.
+- apply eventually_later; auto. intros t s' ST. destruct (H2 t s' ST) as [U V]. auto.
+Qed.
+
+Corollary eventually_implies: forall ge n s (P1 P2: state -> Prop),
+  eventually ge n s P1 ->
+  (forall s, P1 s -> P2 s) ->
+  eventually ge n s P2.
+Proof.
+  intros. replace n with (n + 0)%nat by lia. eapply eventually_trans; eauto using eventually_now.
+Qed.
+
+Lemma eventually_and_invariant: forall ge (Inv: state -> Prop) n s P,
+  (forall s t s', step ge s t s' -> Inv s -> Inv s') ->
+  eventually ge n s P -> Inv s ->
+  eventually ge n s (fun s' => P s' /\ Inv s').
+Proof.
+  intros. revert n s H0 H1. induction n; intros s EV IV; inv EV.
+- apply eventually_now. auto.
+- apply eventually_later; auto. intros. edestruct H2; eauto. 
+Qed.
+
+End CLOSURES.
+          
 Notation " 'Step' L " := (step L (globalenv L)) (at level 1) : closed_smallstep_scope.
 Notation " 'Star' L " := (star (step L) (globalenv L)) (at level 1) : closed_smallstep_scope.
 Notation " 'Plus' L " := (plus (step L) (globalenv L)) (at level 1) : closed_smallstep_scope.
 Notation " 'Forever_silent' L " := (forever_silent (step L) (globalenv L)) (at level 1) : closed_smallstep_scope.
 Notation " 'Forever_reactive' L " := (forever_reactive (step L) (globalenv L)) (at level 1) : closed_smallstep_scope.
 Notation " 'Nostep' L " := (nostep (step L) (globalenv L)) (at level 1) : closed_smallstep_scope.
-Notation " 'Eventually' L " := (eventually (step L) (at_external L) (final_state L) (globalenv L)) (at level 1) : closed_smallstep_scope.
+Notation " 'Eventually' L " := (eventually (step L) (final_state L) (globalenv L)) (at level 1) : closed_smallstep_scope.
 Open Scope closed_smallstep_scope.
 
 
@@ -124,8 +182,8 @@ Record fsim_properties (L1 L2: semantics) (index: Type)
       exists i', exists s2',
          (Plus L2 s2 t s2' \/ (Star L2 s2 t s2' /\ order i' i))
       /\ match_states i' s1' s2';
-    (* fsim_public_preserved:
-      forall id, Genv.public_symbol (symbolenv L2) id = Genv.public_symbol (symbolenv L1) id *)
+    fsim_public_preserved:
+      forall id, Genv.public_symbol (symbolenv L2) id = Genv.public_symbol (symbolenv L1) id
   }.
 
 Arguments fsim_properties: clear implicits.
@@ -138,6 +196,684 @@ Inductive forward_simulation (L1 L2: semantics) : Prop :=
 
 Arguments Forward_simulation {L1 L2 index} order match_states props.
 
+(** An alternate form of the simulation diagram *)
+
+Lemma fsim_simulation':
+  forall L1 L2 index order match_states, fsim_properties L1 L2 index order match_states ->
+  forall i s1 t s1', Step L1 s1 t s1' ->
+  forall s2, match_states i s1 s2 ->
+  (exists i', exists s2', Plus L2 s2 t s2' /\ match_states i' s1' s2')
+  \/ (exists i', order i' i /\ t = E0 /\ match_states i' s1' s2).
+Proof.
+  intros. exploit fsim_simulation; eauto.
+  intros [i' [s2' [A B]]]. intuition.
+  left; exists i'; exists s2'; auto.
+  inv H3.
+  right; exists i'; auto.
+  left; exists i'; exists s2'; split; auto. econstructor; eauto.
+Qed.
+
+(** ** Forward simulation diagrams. *)
+
+(** Various simulation diagrams that imply forward simulation *)
+
+Section FORWARD_SIMU_DIAGRAMS.
+
+Variable L1: semantics.
+Variable L2: semantics.
+
+Hypothesis public_preserved:
+  forall id, Genv.public_symbol (symbolenv L2) id = Genv.public_symbol (symbolenv L1) id.
+
+Variable match_states: state L1 -> state L2 -> Prop.
+
+Hypothesis match_initial_states:
+  forall s1, initial_state L1 s1 ->
+  exists s2, initial_state L2 s2 /\ match_states s1 s2.
+
+Hypothesis match_final_states:
+  forall s1 s2 r,
+  match_states s1 s2 ->
+  final_state L1 s1 r ->
+  final_state L2 s2 r.
+
+(** Simulation when one transition in the first program
+    corresponds to zero, one or several transitions in the second program.
+    However, there is no stuttering: infinitely many transitions
+    in the source program must correspond to infinitely many
+    transitions in the second program. *)
+
+Section SIMULATION_STAR_WF.
+
+(** [order] is a well-founded ordering associated with states
+  of the first semantics.  Stuttering steps must correspond
+  to states that decrease w.r.t. [order]. *)
+
+Variable order: state L1 -> state L1 -> Prop.
+Hypothesis order_wf: well_founded order.
+
+Hypothesis simulation:
+  forall s1 t s1', Step L1 s1 t s1' ->
+  forall s2, match_states s1 s2 ->
+  exists s2',
+  (Plus L2 s2 t s2' \/ (Star L2 s2 t s2' /\ order s1' s1))
+  /\ match_states s1' s2'.
+
+Lemma forward_simulation_star_wf: forward_simulation L1 L2.
+Proof.
+  apply Forward_simulation with order (fun idx s1 s2 => idx = s1 /\ match_states s1 s2);
+  constructor.
+- auto.
+- intros. exploit match_initial_states; eauto. intros [s2 [A B]].
+    exists s1; exists s2; auto.
+- intros. destruct H. eapply match_final_states; eauto.
+- intros. destruct H0. subst i. exploit simulation; eauto. intros [s2' [A B]].
+  exists s1'; exists s2'; intuition auto.
+- auto.
+Qed.
+
+End SIMULATION_STAR_WF.
+
+Section SIMULATION_STAR.
+
+(** We now consider the case where we have a nonnegative integer measure
+  associated with states of the first semantics.  It must decrease when we take
+  a stuttering step. *)
+
+Variable measure: state L1 -> nat.
+
+Hypothesis simulation:
+  forall s1 t s1', Step L1 s1 t s1' ->
+  forall s2, match_states s1 s2 ->
+  (exists s2', Plus L2 s2 t s2' /\ match_states s1' s2')
+  \/ (measure s1' < measure s1 /\ t = E0 /\ match_states s1' s2)%nat.
+
+Lemma forward_simulation_star: forward_simulation L1 L2.
+Proof.
+  apply forward_simulation_star_wf with (ltof _ measure).
+  apply well_founded_ltof.
+  intros. exploit simulation; eauto. intros [[s2' [A B]] | [A [B C]]].
+  exists s2'; auto.
+  exists s2; split. right; split. rewrite B. apply star_refl. auto. auto.
+Qed.
+
+End SIMULATION_STAR.
+
+(** Simulation when one transition in the first program corresponds
+    to one or several transitions in the second program. *)
+
+Section SIMULATION_PLUS.
+
+Hypothesis simulation:
+  forall s1 t s1', Step L1 s1 t s1' ->
+  forall s2, match_states s1 s2 ->
+  exists s2', Plus L2 s2 t s2' /\ match_states s1' s2'.
+
+Lemma forward_simulation_plus: forward_simulation L1 L2.
+Proof.
+  apply forward_simulation_star with (measure := fun _ => O).
+  intros. exploit simulation; eauto.
+Qed.
+
+End SIMULATION_PLUS.
+
+(** Lock-step simulation: each transition in the first semantics
+    corresponds to exactly one transition in the second semantics. *)
+
+Section SIMULATION_STEP.
+
+Hypothesis simulation:
+  forall s1 t s1', Step L1 s1 t s1' ->
+  forall s2, match_states s1 s2 ->
+  exists s2', Step L2 s2 t s2' /\ match_states s1' s2'.
+
+Lemma forward_simulation_step: forward_simulation L1 L2.
+Proof.
+  apply forward_simulation_plus.
+  intros. exploit simulation; eauto. intros [s2' [A B]].
+  exists s2'; split; auto. apply plus_one; auto.
+Qed.
+
+End SIMULATION_STEP.
+
+(** Simulation when one transition in the first program
+    corresponds to zero or one transitions in the second program.
+    However, there is no stuttering: infinitely many transitions
+    in the source program must correspond to infinitely many
+    transitions in the second program. *)
+
+Section SIMULATION_OPT.
+
+Variable measure: state L1 -> nat.
+
+Hypothesis simulation:
+  forall s1 t s1', Step L1 s1 t s1' ->
+  forall s2, match_states s1 s2 ->
+  (exists s2', Step L2 s2 t s2' /\ match_states s1' s2')
+  \/ (measure s1' < measure s1 /\ t = E0 /\ match_states s1' s2)%nat.
+
+Lemma forward_simulation_opt: forward_simulation L1 L2.
+Proof.
+  apply forward_simulation_star with measure.
+  intros. exploit simulation; eauto. intros [[s2' [A B]] | [A [B C]]].
+  left; exists s2'; split; auto. apply plus_one; auto.
+  right; auto.
+Qed.
+
+End SIMULATION_OPT.
+
+End FORWARD_SIMU_DIAGRAMS.
+
+
+(** ** Forward simulation with the "eventually" modality *)
+
+(** A forward simulation diagram where the first semantics can take some extra steps
+    before reaching a state that restores the simulation relation. *)
+
+Section FORWARD_SIMU_EVENTUALLY.
+
+Variable L1: semantics.
+Variable L2: semantics.
+Variable index: Type.
+Variable order: index -> index -> Prop.
+Variable match_states: index -> state L1 -> state L2 -> Prop.
+
+Hypothesis order_wf: well_founded order.
+Hypothesis initial_states:
+  forall s1, initial_state L1 s1 ->
+  exists i, exists s2, initial_state L2 s2 /\ match_states i s1 s2.
+Hypothesis final_states:
+  forall i s1 s2 r,
+    match_states i s1 s2 -> final_state L1 s1 r -> final_state L2 s2 r.
+
+Hypothesis simulation:
+  forall s1 t s1', Step L1 s1 t s1' ->
+  forall i s2, match_states i s1 s2 ->
+  exists n i' s2',
+     (Plus L2 s2 t s2' \/ (Star L2 s2 t s2' /\ order i' i))
+     /\ Eventually L1 n s1' (fun s1'' => match_states i' s1'' s2').
+
+Hypothesis public_preserved:
+  forall id, Genv.public_symbol (symbolenv L2) id = Genv.public_symbol (symbolenv L1) id.
+
+Lemma forward_simulation_eventually: forward_simulation L1 L2.
+Proof.
+  apply @Forward_simulation with
+    (index := (index * nat)%type)
+    (order := lex_ord order Nat.lt)
+    (match_states := fun i s1 s2 => Eventually L1 (snd i) s1 (fun s1'' => match_states (fst i) s1'' s2)).
+  constructor.
+- apply wf_lex_ord; auto using lt_wf.
+- intros. exploit initial_states; eauto. intros (i & s2 & A & B).
+  exists (i, O), s2; auto using eventually_now.
+- intros [i n] s1 s2 r EV FS; simpl in *. inv EV.
+  + eapply final_states; eauto.
+  + eelim H; eauto.
+- intros s1 t s1' ST [i n] s2 EV; simpl in *. inv EV.
+  + exploit simulation; eauto. intros (n & i' & s2' & A & B).
+    exists (i', n), s2'; split; auto.
+    destruct A as [P | [P Q]]; auto using lex_ord_left.
+  + apply H0 in ST. destruct ST as (A & B). subst t.
+    exists (i, n0), s2; split.
+    right; split. apply star_refl. apply lex_ord_right; lia.
+    exact B.
+- apply public_preserved.
+Qed.
+
+End FORWARD_SIMU_EVENTUALLY.
+
+(** Two simplified diagrams. *)
+
+Section FORWARD_SIMU_EVENTUALLY_SIMPL.
+
+Variable L1: semantics.
+Variable L2: semantics.
+Variable match_states: state L1 -> state L2 -> Prop.
+
+Hypothesis public_preserved:
+  forall id, Genv.public_symbol (symbolenv L2) id = Genv.public_symbol (symbolenv L1) id.
+Hypothesis initial_states:
+  forall s1, initial_state L1 s1 ->
+  exists s2, initial_state L2 s2 /\ match_states s1 s2.
+Hypothesis final_states:
+  forall s1 s2 r,
+  match_states s1 s2 -> final_state L1 s1 r -> final_state L2 s2 r.
+
+(** Simplified "plus" simulation diagram, when L2 always makes at least one transition. *)
+
+Section FORWARD_SIMU_EVENTUALLY_PLUS.
+
+Hypothesis simulation:
+  forall s1 t s1', Step L1 s1 t s1' ->
+  forall s2, match_states s1 s2 ->
+  exists n s2',
+     Plus L2 s2 t s2'
+  /\ Eventually L1 n s1' (fun s1'' => match_states s1'' s2').
+
+Lemma forward_simulation_eventually_plus: forward_simulation L1 L2.
+Proof.
+  apply forward_simulation_eventually with (order := lt) (match_states := fun i s1 s2 => match_states s1 s2).
+- apply lt_wf.
+- intros. exploit initial_states; eauto. intros (s2 & A & B). exists O, s2; auto.
+- intros. eapply final_states; eauto.
+- intros. exploit simulation; eauto. intros (n & s2' & A & B).
+  exists n, O, s2'; auto.
+- auto.
+Qed.
+
+End FORWARD_SIMU_EVENTUALLY_PLUS.
+
+(** Simplified "star" simulation diagram, with a decreasing, well-founded order on L1 states. *)
+
+Section FORWARD_SIMU_EVENTUALLY_STAR_WF.
+
+Variable order: state L1 -> state L1 -> Prop.
+Hypothesis order_wf: well_founded order.
+
+Hypothesis simulation:
+  forall s1 t s1', Step L1 s1 t s1' ->
+  forall s2, match_states s1 s2 ->
+     (exists s2',
+        (Plus L2 s2 t s2' \/ (Star L2 s2 t s2' /\ order s1' s1)) /\ match_states s1' s2')
+  \/ (exists n s2',
+        Plus L2 s2 t s2' /\ Eventually L1 n s1' (fun s1'' => match_states s1'' s2')).
+
+Lemma forward_simulation_eventually_star_wf: forward_simulation L1 L2.
+Proof.
+  apply @Forward_simulation with
+    (index := (nat * state L1)%type)
+    (order := lex_ord Nat.lt order)
+    (match_states := fun i s1 s2 => snd i = s1 /\ Eventually L1 (fst i) s1 (fun s1'' => match_states s1'' s2)).
+  constructor; intros.
+- apply wf_lex_ord; auto using lt_wf.
+- exploit initial_states; eauto. intros (s2 & A & B).
+  exists (O, s1), s2; auto using eventually_now.
+- destruct i as [n s11]; destruct H as [P Q]; simpl in *; subst s11.
+  inv Q.
+  + eapply final_states; eauto.
+  + eelim H; eauto.
+- destruct i as [n s11]; destruct H0 as [P Q]; simpl in *; subst s11.
+  inv Q.
+  + exploit simulation; eauto. intros [(s2' & A & B) | (n & s2' & A & B)].
+    * exists (O, s1'), s2'; split. 
+      destruct A as [A | [A1 A2]]; auto using lex_ord_right.
+      auto using eventually_now.
+    * exists (n, s1'), s2'; auto.
+  + apply H1 in H. destruct H. subst t.
+    exists (n0, s1'), s2; split.
+    right; split. apply star_refl. apply lex_ord_left; lia.
+    auto.
+- auto.
+Qed.
+
+End FORWARD_SIMU_EVENTUALLY_STAR_WF.
+
+(** Simplified "star" simulation diagram, with a decreasing measure on L1 states. *)
+
+Section FORWARD_SIMU_EVENTUALLY_STAR.
+
+Variable measure: state L1 -> nat.
+
+Hypothesis simulation:
+  forall s1 t s1', Step L1 s1 t s1' ->
+  forall s2, match_states s1 s2 ->
+     (exists s2',
+        (Plus L2 s2 t s2' \/ (Star L2 s2 t s2' /\ measure s1' < measure s1))%nat
+        /\ match_states s1' s2')
+  \/ (exists n s2',
+        Plus L2 s2 t s2' /\ Eventually L1 n s1' (fun s1'' => match_states s1'' s2')).
+
+Lemma forward_simulation_eventually_star: forward_simulation L1 L2.
+Proof.
+  apply forward_simulation_eventually_star_wf with (ltof _ measure).
+- apply well_founded_ltof.
+- exact simulation.
+Qed.
+
+End FORWARD_SIMU_EVENTUALLY_STAR.
+
+End FORWARD_SIMU_EVENTUALLY_SIMPL.
+
+(** ** Forward simulation of transition sequences *)
+
+Section SIMULATION_SEQUENCES.
+
+Context L1 L2 index order match_states (S: fsim_properties L1 L2 index order match_states).
+
+Lemma simulation_star:
+  forall s1 t s1', Star L1 s1 t s1' ->
+  forall i s2, match_states i s1 s2 ->
+  exists i', exists s2', Star L2 s2 t s2' /\ match_states i' s1' s2'.
+Proof.
+  induction 1; intros.
+  exists i; exists s2; split; auto. apply star_refl.
+  exploit fsim_simulation; eauto. intros [i' [s2' [A B]]].
+  exploit IHstar; eauto. intros [i'' [s2'' [C D]]].
+  exists i''; exists s2''; split; auto. eapply star_trans; eauto.
+  intuition auto. apply plus_star; auto.
+Qed.
+
+Lemma simulation_plus:
+  forall s1 t s1', Plus L1 s1 t s1' ->
+  forall i s2, match_states i s1 s2 ->
+  (exists i', exists s2', Plus L2 s2 t s2' /\ match_states i' s1' s2')
+  \/ (exists i', clos_trans _ order i' i /\ t = E0 /\ match_states i' s1' s2).
+Proof.
+  induction 1 using plus_ind2; intros.
+(* base case *)
+  exploit fsim_simulation'; eauto. intros [A | [i' A]].
+  left; auto.
+  right; exists i'; intuition auto with sets.
+(* inductive case *)
+  exploit fsim_simulation'; eauto. intros [[i' [s2' [A B]]] | [i' [A [B C]]]].
+  exploit simulation_star. apply plus_star; eauto. eauto.
+  intros [i'' [s2'' [P Q]]].
+  left; exists i''; exists s2''; split; auto. eapply plus_star_trans; eauto.
+  exploit IHplus; eauto. intros [[i'' [s2'' [P Q]]] | [i'' [P [Q R]]]].
+  subst. simpl. left; exists i''; exists s2''; auto.
+  subst. simpl. right; exists i''; intuition auto.
+  eapply t_trans; eauto. eapply t_step; eauto.
+Qed.
+
+Lemma simulation_forever_silent:
+  forall i s1 s2,
+  Forever_silent L1 s1 -> match_states i s1 s2 ->
+  Forever_silent L2 s2.
+Proof.
+  assert (forall i s1 s2,
+          Forever_silent L1 s1 -> match_states i s1 s2 ->
+          forever_silent_N (step L2) order (globalenv L2) i s2).
+    cofix COINDHYP; intros.
+    inv H. destruct (fsim_simulation S _ _ _ H1 _ _ H0) as [i' [s2' [A B]]].
+    destruct A as [C | [C D]].
+    eapply forever_silent_N_plus; eauto.
+    eapply forever_silent_N_star; eauto.
+  intros. eapply forever_silent_N_forever; eauto. eapply fsim_order_wf; eauto.
+Qed.
+
+Lemma simulation_forever_reactive:
+  forall i s1 s2 T,
+  Forever_reactive L1 s1 T -> match_states i s1 s2 ->
+  Forever_reactive L2 s2 T.
+Proof.
+  cofix COINDHYP; intros.
+  inv H.
+  edestruct simulation_star as [i' [st2' [A B]]]; eauto.
+  econstructor; eauto.
+Qed.
+
+End SIMULATION_SEQUENCES.
+
+(** ** Composing two forward simulations *)
+
+Lemma compose_forward_simulations:
+  forall L1 L2 L3, forward_simulation L1 L2 -> forward_simulation L2 L3 -> forward_simulation L1 L3.
+Proof.
+  intros L1 L2 L3 S12 S23.
+  destruct S12 as [index order match_states props].
+  destruct S23 as [index' order' match_states' props'].
+
+  set (ff_index := (index' * index)%type).
+  set (ff_order := lex_ord (clos_trans _ order') order).
+  set (ff_match_states := fun (i: ff_index) (s1: state L1) (s3: state L3) =>
+                             exists s2, match_states (snd i) s1 s2 /\ match_states' (fst i) s2 s3).
+  apply Forward_simulation with ff_order ff_match_states; constructor.
+- (* well founded *)
+  unfold ff_order. apply wf_lex_ord. apply wf_clos_trans.
+  eapply fsim_order_wf; eauto. eapply fsim_order_wf; eauto.
+- (* initial states *)
+  intros. exploit (fsim_match_initial_states props); eauto. intros [i [s2 [A B]]].
+  exploit (fsim_match_initial_states props'); eauto. intros [i' [s3 [C D]]].
+  exists (i', i); exists s3; split; auto. exists s2; auto.
+- (* final states *)
+  intros. destruct H as [s3 [A B]].
+  eapply (fsim_match_final_states props'); eauto.
+  eapply (fsim_match_final_states props); eauto.
+- (* simulation *)
+  intros. destruct H0 as [s3 [A B]]. destruct i as [i2 i1]; simpl in *.
+  exploit (fsim_simulation' props); eauto. intros [[i1' [s3' [C D]]] | [i1' [C [D E]]]].
++ (* L2 makes one or several steps. *)
+  exploit simulation_plus; eauto. intros [[i2' [s2' [P Q]]] | [i2' [P [Q R]]]].
+* (* L3 makes one or several steps *)
+  exists (i2', i1'); exists s2'; split. auto. exists s3'; auto.
+* (* L3 makes no step *)
+  exists (i2', i1'); exists s2; split.
+  right; split. subst t; apply star_refl. red. left. auto.
+  exists s3'; auto.
++ (* L2 makes no step *)
+  exists (i2, i1'); exists s2; split.
+  right; split. subst t; apply star_refl. red. right. auto.
+  exists s3; auto.
+- (* symbols *)
+  intros. transitivity (Genv.public_symbol (symbolenv L2) id); eapply fsim_public_preserved; eauto.
+Qed.
+
+(** * Receptiveness and determinacy *)
+
+Definition single_events (L: semantics) : Prop :=
+  forall s t s', Step L s t s' -> (length t <= 1)%nat.
+
+Record receptive (L: semantics) : Prop :=
+  Receptive {
+    sr_receptive: forall s t1 s1 t2,
+      Step L s t1 s1 -> match_traces (symbolenv L) t1 t2 -> exists s2, Step L s t2 s2;
+    sr_traces:
+      single_events L
+  }.
+
+Record determinate (L: semantics) : Prop :=
+  Determinate {
+    sd_determ: forall s t1 s1 t2 s2,
+      Step L s t1 s1 -> Step L s t2 s2 ->
+      match_traces (symbolenv L) t1 t2 /\ (t1 = t2 -> s1 = s2);
+    sd_traces:
+      single_events L;
+    sd_initial_determ: forall s1 s2,
+      initial_state L s1 -> initial_state L s2 -> s1 = s2;
+    sd_final_nostep: forall s r,
+      final_state L s r -> Nostep L s;
+    sd_final_determ: forall s r1 r2,
+      final_state L s r1 -> final_state L s r2 -> r1 = r2
+  }.
+
+Section DETERMINACY.
+
+Variable L: semantics.
+Hypothesis DET: determinate L.
+
+Lemma sd_determ_1:
+  forall s t1 s1 t2 s2,
+  Step L s t1 s1 -> Step L s t2 s2 -> match_traces (symbolenv L) t1 t2.
+Proof.
+  intros. eapply sd_determ; eauto.
+Qed.
+
+Lemma sd_determ_2:
+  forall s t s1 s2,
+  Step L s t s1 -> Step L s t s2 -> s1 = s2.
+Proof.
+  intros. eapply sd_determ; eauto.
+Qed.
+
+Lemma sd_determ_3:
+  forall s t s1 s2,
+  Step L s t s1 -> Step L s E0 s2 -> t = E0 /\ s1 = s2.
+Proof.
+  intros. exploit (sd_determ DET). eexact H. eexact H0.
+  intros [A B]. inv A. auto.
+Qed.
+
+Lemma star_determinacy:
+  forall s t s', Star L s t s' ->
+  forall s'', Star L s t s'' -> Star L s' E0 s'' \/ Star L s'' E0 s'.
+Proof.
+  induction 1; intros.
+  auto.
+  inv H2.
+  right. eapply star_step; eauto.
+  exploit sd_determ_1. eexact H. eexact H3. intros MT.
+  exploit (sd_traces DET). eexact H. intros L1.
+  exploit (sd_traces DET). eexact H3. intros L2.
+  assert (t1 = t0 /\ t2 = t3).
+    destruct t1. inv MT. auto.
+    destruct t1; simpl in L1; try extlia.
+    destruct t0. inv MT. destruct t0; simpl in L2; try extlia.
+    simpl in H5. split. congruence. congruence.
+  destruct H1; subst.
+  assert (s2 = s4) by (eapply sd_determ_2; eauto). subst s4.
+  auto.
+Qed.
+
+End DETERMINACY.
+
+(** Extra simulation diagrams for determinate languages. *)
+
+Section FORWARD_SIMU_DETERM.
+
+Variable L1: semantics.
+Variable L2: semantics.
+
+Hypothesis L1det: determinate L1.
+
+Variable index: Type.
+Variable order: index -> index -> Prop.
+Hypothesis wf_order: well_founded order.
+
+Variable match_states: index -> state L1 -> state L2 -> Prop.
+
+Hypothesis match_initial_states:
+  forall s1, initial_state L1 s1 ->
+  exists i s2, initial_state L2 s2 /\ match_states i s1 s2.
+
+Hypothesis match_final_states:
+  forall i s1 s2 r,
+  match_states i s1 s2 ->
+  final_state L1 s1 r ->
+  final_state L2 s2 r.
+
+Hypothesis simulation:
+  forall s1 t s1', Step L1 s1 t s1' ->
+  forall i s2, match_states i s1 s2 ->
+  exists s1'' i' s2',
+      Star L1 s1' E0 s1''
+   /\ (Plus L2 s2 t s2' \/ (Star L2 s2 t s2' /\ order i' i))
+   /\ match_states i' s1'' s2'.
+
+Hypothesis public_preserved:
+  forall id, Genv.public_symbol (symbolenv L2) id = Genv.public_symbol (symbolenv L1) id.
+
+Lemma star_match_eventually:
+  forall s1 s1', Star L1 s1 E0 s1' ->
+  forall i s2, match_states i s1' s2 ->
+  exists n, Eventually L1 n s1 (fun s1'' => match_states i s1'' s2).
+Proof.
+  intros s10 s10' STAR0. pattern s10, s10'; eapply star_E0_ind; eauto.
+  - intros s1 i s2 M. exists O; constructor; auto.
+  - intros s1 s1' s1'' STEP IH i s2 M.
+    destruct (IH i s2 M) as (n & MS).
+    exists (S n); constructor.
+    + intros; red; intros. eapply (sd_final_nostep L1det); eauto.
+    + intros. exploit (sd_determ_3 L1det). eexact H. eexact STEP. intros [A B].
+      subst t s'. auto.
+Qed.
+
+Lemma forward_simulation_determ: forward_simulation L1 L2.
+Proof.
+  apply forward_simulation_eventually with (order := order) (match_states := match_states); auto.
+  intros. exploit simulation; eauto. intros (s1'' & i' & s2' & A & B & C).
+  exploit star_match_eventually; eauto. intros (n & D).
+  exists n, i', s2'; auto.
+Qed.
+
+End FORWARD_SIMU_DETERM.
+
+(** A few useful special cases. *)
+
+Section FORWARD_SIMU_DETERM_DIAGRAMS.
+
+Variable L1: semantics.
+Variable L2: semantics.
+
+Hypothesis L1det: determinate L1.
+
+Variable match_states: state L1 -> state L2 -> Prop.
+
+Hypothesis public_preserved:
+  forall id, Genv.public_symbol (symbolenv L2) id = Genv.public_symbol (symbolenv L1) id.
+
+Hypothesis match_initial_states:
+  forall s1, initial_state L1 s1 ->
+  exists s2, initial_state L2 s2 /\ match_states s1 s2.
+
+Hypothesis match_final_states:
+  forall s1 s2 r,
+  match_states s1 s2 ->
+  final_state L1 s1 r ->
+  final_state L2 s2 r.
+
+Section SIMU_DETERM_STAR.
+
+Variable measure: state L1 -> nat.
+
+Hypothesis simulation:
+  forall s1 t s1', Step L1 s1 t s1' ->
+  forall s2, match_states s1 s2 ->
+  exists s1'' s2',
+      Star L1 s1' E0 s1''
+   /\ (Plus L2 s2 t s2' \/ (Star L2 s2 t s2' /\ measure s1'' < measure s1))%nat
+   /\ match_states s1'' s2'.
+
+Lemma forward_simulation_determ_star: forward_simulation L1 L2.
+Proof.
+  apply forward_simulation_determ with
+    (match_states := fun i s1 s2 => i = s1 /\ match_states s1 s2)
+    (order := ltof _ measure).
+- assumption.
+- apply well_founded_ltof.
+- intros. exploit match_initial_states; eauto. intros (s2 & A & B). 
+  exists s1, s2; auto.
+- intros. destruct H. eapply match_final_states; eauto.
+- intros. destruct H0; subst i. 
+  exploit simulation; eauto. intros (s1'' & s2' & A & B & C).
+  exists s1'', s1'', s2'. auto.
+- assumption.
+Qed.
+
+End SIMU_DETERM_STAR.
+
+Section SIMU_DETERM_PLUS.
+
+Hypothesis simulation:
+  forall s1 t s1', Step L1 s1 t s1' ->
+  forall s2, match_states s1 s2 ->
+  exists s1'' s2', Star L1 s1' E0 s1'' /\ Plus L2 s2 t s2' /\ match_states s1'' s2'.
+
+Lemma forward_simulation_determ_plus: forward_simulation L1 L2.
+Proof.
+  apply forward_simulation_determ_star with (measure := fun _ => O).
+  intros. exploit simulation; eauto. intros (s1'' & s2' & A & B & C).
+  exists s1'', s2'; auto.
+Qed.
+
+End SIMU_DETERM_PLUS.
+
+Section SIMU_DETERM_ONE.
+
+Hypothesis simulation:
+  forall s1 t s1', Step L1 s1 t s1' ->
+  forall s2, match_states s1 s2 ->
+  exists s1'' s2', Star L1 s1' E0 s1'' /\ Step L2 s2 t s2' /\ match_states s1'' s2'.
+
+Lemma forward_simulation_determ_one: forward_simulation L1 L2.
+Proof.
+  apply forward_simulation_determ_plus.
+  intros. exploit simulation; eauto. intros (s1'' & s2' & A & B & C).
+  exists s1'', s2'; auto using plus_one.
+Qed.
+
+End SIMU_DETERM_ONE.
+
+End FORWARD_SIMU_DETERM_DIAGRAMS.
 
 Definition safe (L: semantics) (s: state L) : Prop :=
   forall s',
@@ -176,8 +912,8 @@ Record bsim_properties (L1 L2: semantics) (index: Type)
       exists i', exists s1',
          (Plus L1 s1 t s1' \/ (Star L1 s1 t s1' /\ order i' i))
       /\ match_states i' s1' s2';
-    (* bsim_public_preserved:
-      forall id, Genv.public_symbol (symbolenv L2) id = Genv.public_symbol (symbolenv L1) id *)
+    bsim_public_preserved:
+      forall id, Genv.public_symbol (symbolenv L2) id = Genv.public_symbol (symbolenv L1) id
   }.
 
 Arguments bsim_properties: clear implicits.
@@ -263,6 +999,7 @@ Proof.
   intros i s1' s2' r MS (r1 & R1 & FINAL).
   exploit fsim_match_final_states0; eauto. intros (r2 & FINAL' & MATCH_REPLY).
   eexists. split; eauto.
+  eapply match_senv_public_preserved; eauto.
 Qed.
 
 End FORWARD.
@@ -311,6 +1048,7 @@ Proof.
 
   intros. apply safe_sound_1 in H1.
   eapply bsim_simulation0; eauto.
+  eapply  match_senv_public_preserved; eauto.
 Qed.
 
 End BACKWARD.
